DataflowToClight.v
@@ -1,44 +1,22 @@
 Require Import Rustre.Common.
-Require Import Rustre.Dataflow.
-Require Import Rustre.Dataflow.IsFree.Decide.
-Require Import Rustre.Dataflow.WellFormed.Decide.
-Require Import Rustre.ObcToClight.Interface.
-Require Import Rustre.DataflowToObc.Translation.
+Require Import Rustre.Ident.
 Require Import Rustre.ObcToClight.Translation.
-Require Import Rustre.Obc.FuseIfte.
 
 Require Import common.Errors.
-Require Import Rustre.Operators.
-Require Import Rustre.Ident.
 
-Module Export OpAux := OperatorsAux Op.
-
-Module Import SynDF := Dataflow.Syntax.SyntaxFun Ids Op.
-Module Import SynObc := ObcToClight.Translation.Syn.
-Module Import Mem := Dataflow.Memories.MemoriesFun Ids Op SynDF.
-Module Import DF2ObcTrans := TranslationFun Ids Op OpAux SynDF SynObc Mem.
-
-Module Import IsF := IsFreeFun Ids Op SynDF.
-Module Import IsFDec := Dataflow.IsFree.Decide.Decide Ids Op SynDF IsF.
-Module Import Ord := OrderedFun Ids Op SynDF.
-Module Import IsD := IsDefined Ids Op SynDF Mem.
-Module Import IsV := IsVariableFun Ids Op SynDF Mem IsD.
-Module Import IsDDec := IsDefined.Decide.Decide Ids Op SynDF Mem IsD.
-Module Import IsVDec := IsVariable.Decide.Decide Ids Op SynDF Mem IsD IsV.
-Module Import NoD := NoDupFun Ids Op SynDF Mem IsD IsV.
-Module Import Wef := WellFormedFun Ids Op SynDF IsF Ord Mem IsD IsV NoD.
-Module Import WefD := Dataflow.WellFormed.Decide.Decide
-                        Ids Op SynDF IsF IsFDec Ord Mem IsD IsV IsDDec IsVDec NoD Wef.
-
-Module Import SemObc := Rustre.Obc.Semantics.SemanticsFun Ids Op OpAux SynObc.
-Module Import Equ := Rustre.Obc.Equiv.EquivFun Ids Op OpAux SynObc SemObc.
-Module Import FuseIFTE := FuseIfteFun Ids Op OpAux SynDF SynObc SemObc Equ.
+Require Import Rustre.Instantiator.
+Import DF.Syn.
+Import WeFDec.
+Import DF.Mem.
+Import Obc.Syn.
+Import Fus.
+Import Trans.
 
 Require Import String.
 
 Open Scope error_monad_scope.
 
-Definition is_well_sch (res: Errors.res unit) (n: node) :=
+Definition is_well_sch (res: res unit) (n: node) :=
   match res with
   | OK _ =>
     let eqs := n.(n_eqs) in
@@ -47,7 +25,6 @@ Definition is_well_sch (res: Errors.res unit) (n: node) :=
     else Error (Errors.msg ("node " ++ pos_to_str n.(n_name) ++ " is not well scheduled."))
   | _ => res
   end.
-
 
 Definition fuse_method (m: method): method :=
   match m with
@@ -81,4 +58,4 @@ Definition fuse_class (c: class): class :=
 
 Definition compile (g: global) (main_node: ident) :=
   do _ <- (List.fold_left is_well_sch g (OK tt));
-  ObcToClight.Translation.translate (List.map fuse_class (DF2ObcTrans.translate g)) main_node.
+  ObcToClight.Translation.translate (List.map fuse_class (Trans.translate g)) main_node.
