Instantiator.v
@@ -13,6 +13,9 @@ Require Import Obc.
 Require Import DataflowToObc.Translation.
 Require Import Dataflow.Memories.
 Require Import Obc.FuseIfte.
+Require Import Dataflow.IsFree.Decide.
+Require Import Dataflow.WellFormed.Decide.
+
 Module DF := DataflowFun Ids Op OpAux.
 Module Obc := ObcFun Ids Op OpAux.
 Module Mem := MemoriesFun Ids Op DF.Syn.
@@ -21,3 +24,5 @@ Module IsP := IsPresentFun Ids Op OpAux DF.Syn Obc.Syn Obc.Sem Mem Trans.
 Module MemCor := MemoryCorresFun Ids Op OpAux DF Obc.
 Module Fus := FuseIfteFun Ids Op OpAux DF.Syn Obc.Syn Obc.Sem Obc.Equ.
 Module Corr := DataflowToObc.Correctness.CorrectnessFun Ids Op OpAux DF Obc Mem Trans IsP MemCor Fus.
+
+Module WeFDec := WellFormed.Decide.Decide Ids Op DF.Syn DF.IsF DF.IsFDec DF.Ord DF.Mem DF.IsD DF.IsV DF.IsDDec DF.IsVDec DF.NoD DF.WeF.
